\documentclass[14pt,a4paper,final]{article}
\usepackage[utf8]{inputenc}
\usepackage{amsmath}
\usepackage{amsfonts}
\usepackage{amssymb}
\begin{document}
Passive Motion Paradigm Equations\\
\begin{equation}
f(x)=k_{ext}(x_d-x)
\end{equation}
\begin{equation}
\tau=J^Tf(x)
\end{equation}
\begin{equation}
\dot{q}=A_{int}\tau
\end{equation}
\begin{equation}
\dot{x}=J\dot{q}
\end{equation}
\begin{equation}
x(t)=\int J \dot{q} dt
\end{equation}

Equations related to the floating base system\\
Generalized Cooridinates

\[q = \begin{bmatrix}
x_b \\
y_b \\
\theta_b \\
q_1 \\
q_2
\end{bmatrix}
\]

Dynamics, \\

$ M(q)\ddot{q}+C(q,\dot{q})\dot{q}+G(q) = \tau $ \\
\\
$h(q,\dot{q})=C(q,\dot{q})\dot{q}+G(q)$ \\ 
Using the above equation \\
$ M(q)\ddot{q}+h(q,\dot{q}) = \tau $ \\
Control Laws, \\

$ M(q)\ddot{q}+h(q,\dot{q}) - J_1^TF_1 -J_2^TF_2 = 0 $ \\

External Forces, \\

\[F_1 = \begin{bmatrix}
^{1}F_x \\
^{1}F_y \\
^{1}\tau \\
\end{bmatrix}
\]
\[F_2 = \begin{bmatrix}
^{2}F_x \\
^{2}F_y \\
^{2}\tau \\
\end{bmatrix}
\]

Rearranging the control law, 
\[B = \begin{bmatrix}
J_1^T && J_2^T
\end{bmatrix}
\]
\[u = \begin{bmatrix}
F_1 \\
F_2
\end{bmatrix}
\] \\


$ M(q)\ddot{q}+h(q,\dot{q}) = Bu $ \\

States Variables,

\begin{equation}
x_1 = q 
\end{equation}
\begin{equation}
x_2 = \dot{q}
\end{equation}

\[x = \begin{bmatrix}
x_1 \\
x_2
\end{bmatrix}
\] 

\[\dot{x} = \begin{bmatrix}
\dot{x}_1 \\
\dot{x}_2
\end{bmatrix}
\] 

\[\dot{x} = \begin{bmatrix}
x_2 \\
M^{-1}[Bu-h(x_1,x_2)]
\end{bmatrix}
\] 

\[ \dot{x} =
\begin{bmatrix}
x_2 \\
-M^{-1}h(x_1,x_2)
\end{bmatrix} + \begin{bmatrix}
0 \\
M^{-1}B
\end{bmatrix} u
\]

\[\dot{x} = f(x) + g(x)u
\] 


Output Variables \\

\[y = \begin{bmatrix}
x_b \\
y_B \\
\theta_b
\end{bmatrix}
\] 

\[y = \begin{bmatrix}
q_1 \\
q_2 \\
\end{bmatrix}
\]

Output Equation,
\begin{equation}
\dot{y} = S\dot{q}
\end{equation} 

\begin{equation}
\ddot{y} = S\ddot{q} \Rightarrow SM^{-1}[Bu-h]
\end{equation}

\begin{equation}
\ddot{y} = -SM^{-1}h + SM^{-1}B u
\end{equation}

\begin{equation}
\ddot{y} = h(u)
\end{equation}

Considering the joint constraints,
Control Laws, \\

$ M(q)\ddot{q}+h(q,\dot{q}) - J_1^TF_1 -J_2^TF_2 -J_c^TF_c = 0 $ \\

$ M(q)\ddot{q}+h(q,\dot{q}) = Bu + J_c^TF_c$ \\

Estimating constraint forces, \\

$J_c\ddot{q} = 0 \Rightarrow J_c M^{-1}[Bu + J_c^TF_c-h] = 0$ \\

$F_c = (J_cM^{-1}J_c^T)^{-1}J_cM^{-1}[h-Bu]$

\end{document}